use nlist_sorted

src/cbor/pulse/raw/everparse/CBOR.Pulse.Raw.Format.Parse.fst
@@ -175,43 +175,10 @@ fn cbor_raw_ints_optimal (_: unit) : LowParse.Pulse.Recursive.impl_pred_t #_ #_ 
 }
 ```
 
-let impl_order_t
-  (#t: Type0)
-  (#k: parser_kind)
-  (#p: parser k t)
-  (s: serializer p)
-  (order: (t -> t -> bool))
-=
-    (a1: slice byte) ->
-    (a2: slice byte) ->
-    (#p1: perm) ->
-    (#p2: perm) ->
-    (#v1: Ghost.erased t) ->
-    (#v2: Ghost.erased t) ->
-    stt bool
-      (pts_to_serialized s a1 #p1 v1 ** pts_to_serialized s a2 #p2 v2)
-      (fun res -> pts_to_serialized s a1 #p1 v1 ** pts_to_serialized s a2 #p2 v2 ** pure (res == order v1 v2))
-
-assume val nlist_sorted
-  (#t: Type0)
-  (#k: Ghost.erased parser_kind)
-  (#p: parser k t)
-  (s: serializer p)
-  (sq: squash (k.parser_kind_subkind == Some ParserStrong))
-  (order: Ghost.erased (t -> t -> bool))
-  (impl_order: impl_order_t s order)
-  (n: SZ.t)
-  (a: slice byte)
-  (#pm: perm)
-  (#v: Ghost.erased (LowParse.Spec.VCList.nlist (SZ.v n) t))
-: stt bool
-    (pts_to_serialized (LowParse.Spec.VCList.serialize_nlist (SZ.v n) s) a #pm v)
-    (fun res -> pts_to_serialized (LowParse.Spec.VCList.serialize_nlist (SZ.v n) s) a #pm v ** pure (res == List.Tot.sorted order v))
-
-assume val impl_deterministically_encoded_cbor_map_key_order : impl_order_t (LowParse.Pulse.Combinators.serialize_nondep_then serialize_raw_data_item serialize_raw_data_item) (map_entry_order deterministically_encoded_cbor_map_key_order raw_data_item)
+assume val impl_deterministically_encoded_cbor_map_key_order : LowParse.Pulse.VCList.impl_order_t (LowParse.Pulse.Combinators.serialize_nondep_then serialize_raw_data_item serialize_raw_data_item) (map_entry_order deterministically_encoded_cbor_map_key_order raw_data_item)
 
 ```pulse
-fn cbor_raw_sorted (_: squash SZ.fits_u64) : LowParse.Pulse.Recursive.impl_pred_t #_ #_ #_ serialize_raw_data_item (R.raw_data_item_sorted_elem deterministically_encoded_cbor_map_key_order)
+fn cbor_raw_sorted (sq: squash SZ.fits_u64) : LowParse.Pulse.Recursive.impl_pred_t #_ #_ #_ serialize_raw_data_item (R.raw_data_item_sorted_elem deterministically_encoded_cbor_map_key_order)
 = (a: _)
   (#pm: _)
   (#va: _)
@@ -247,7 +214,7 @@ fn cbor_raw_sorted (_: squash SZ.fits_u64) : LowParse.Pulse.Recursive.impl_pred_
           (LowParse.Spec.VCList.serialize_nlist (SZ.v (SZ.uint64_to_sizet n)) s)
           ap;
         Trade.trans _ _ (pts_to_serialized serialize_raw_data_item a #pm va);
-        let res = nlist_sorted s () (map_entry_order deterministically_encoded_cbor_map_key_order raw_data_item) (impl_deterministically_encoded_cbor_map_key_order) (SZ.uint64_to_sizet n) ap;
+        let res = LowParse.Pulse.VCList.nlist_sorted s () (LowParse.Pulse.Combinators.jump_nondep_then (jump_raw_data_item sq) (jump_raw_data_item sq)) (map_entry_order deterministically_encoded_cbor_map_key_order raw_data_item) (impl_deterministically_encoded_cbor_map_key_order) (SZ.uint64_to_sizet n) ap;
         Trade.elim _ _;
         res
       } else {
